Fix proofs up to clos_known

compiler/backend/semantics/closPropsScript.sml
@@ -2137,12 +2137,13 @@ Theorem simple_val_rel_do_app
 val simple_compile_state_rel_def = Define `
   simple_compile_state_rel vr sr comp cr <=>
     simple_state_rel vr sr /\
-    (! p exps res. comp p = (exps, res) ==> res = [] /\
-        LENGTH exps = LENGTH (FST p) /\ cr (FST p) exps) /\
     (! (s:('c, 'ffi) closSem$state) (t:('c, 'ffi) closSem$state).
         sr s t ==>
         t.clock = s.clock /\ s.compile = pure_cc comp t.compile /\
         t.compile_oracle = pure_co comp o s.compile_oracle /\
+        (! n exps res p aux. SND (s.compile_oracle n) = (p, aux) ==>
+            comp (p, aux) = (exps, res) ==>
+            res = [] /\ LENGTH exps = LENGTH p /\ cr p exps) /\
         (!n. SND (SND (s.compile_oracle n)) = []) /\
         (! n. sr (s with <| clock := n; compile_oracle :=
                         shift_seq 1 s.compile_oracle; code := s.code |>)
@@ -2217,7 +2218,8 @@ Proof
   \\ rpt (TYPE_CASE_TAC "list" \\ fs [])
   \\ imp_res_tac simple_val_rel_v_to_bytes
   \\ imp_res_tac simple_val_rel_v_to_words
-  \\ FIRST_X_ASSUM (qspec_then `SND (s.compile_oracle 0)` ASSUME_TAC)
+  \\ Cases_on `SND (s.compile_oracle 0)`
+  \\ FIRST_X_ASSUM drule \\ rfs [] \\ rveq
   \\ rfs [pure_co_def, EVAL ``shift_seq k s 0``, pure_cc_def]
   \\ EVERY_CASE_TAC \\ rfs [] \\ fs [finite_mapTheory.FUPDATE_LIST_THM]
 QED
